src/basic/FStarC.Options.fsti
@@ -204,6 +204,10 @@ val codegen                     : unit    -> ML (option codegen_t)
 val codegen_libs                : unit    -> ML (list (list string))
 val custard_entries             : unit    -> ML (list string)
 val custard_dump_ir             : unit    -> ML bool
+val custard_dump_specializations: unit    -> ML bool
+val custard_fuel                : unit    -> ML int
+val custard_max_specializations : unit    -> ML int
+val custard_monomorphize_types  : unit    -> ML bool
 
 val profile_group_by_decl       : unit    -> ML bool
 
